## Boolean Algebra Theorems
$$ x+0=x $$
$$ x+y=y+x $$
$$ x\cdot 1=x $$
$$ x\cdot y=y\cdot x $$
$$ x\cdot(y+z) = (x\cdot y)+(x\cdot z) $$
$$ x+(y\cdot z) = (x+y)\cdot(x+z) $$
$$ x+\bar x = 1 $$
$$ x\cdot\bar x = 0 $$
$$ x+1 = 1 $$
$$ x\cdot 0 = 0 $$
$$ x+x = x $$
$$ x\cdot x = x $$
$$ \bar{(\bar x)} = x $$
$$ x+(y+z) = (x+y)+z $$
$$ x\cdot(y\cdot z) = (x\cdot y)\cdot z $$
$$ \bar{(x+y)} = (\bar x\cdot\bar y) $$
$$ \bar{(x\cdot y)} = \bar x + \bar y $$
$$ x+(x\cdot y) = x $$
$$ x\cdot(x+y) = x $$
