1. $x^2y''-2y = 0$
$y = x^m$
$y' = mx^{m-1}$
$y'' = m(m-1)x^{m-2}$
$$ x^{\cancel2}x^{m\cancel{-2}}m(m-1) - 2x^m = 0 $$
$$ x^m (m^2-m-2) = 0 \quad=>\quad m^2-m-2=0 $$
$$ (m-2)(m+1)=0 $$
$m_1 = 2$
$m_2 = -1$
$$ y(x) = C_1x^{2} + C_2x^{-1} $$
3. $xy''+y' = 0$
$y = x^m$
$y' = mx^{m-1}$
$y'' = m(m-1)x^{m-2}$
$$ x^{m-1}(m^2-m) + mx^{m-1}=0 $$
$$ x^{m-1}(m^2) $$
$m_1 = m_2 = 0$
$$ y(x) = C_1 + C_2\ln|x| $$
5. $x^2y''+xy'+4y=0$
$$ x^m(m^2-m)+x^m(m)+x^m(4) = 0 $$
$$ m^2 + 4 = 0 $$
$m = \pm 2i$
$$ y(x) = C_1\cos(2\ln|x|) + C_2\sin(2\ln|x|) $$
7. $x^2y''-3xy'-2y=0$
$$ x^m(m^2-m)-3mx^m -2x^m $$
$$ m^2-4m-2 = 0 $$
$$ = \frac{4\pm\sqrt{16-4(1)(-2)}}{2(1)} = \frac{4\pm\sqrt{24}}{2} $$
$$ = 2+\sqrt6 \qquad = 2-\sqrt 6 $$
$$ y(x) = C_1x^{2+\sqrt 6} + C_2x^{2-\sqrt 6} $$
