### Section 9.16, Problem 2
verify the divergence theorem.

$F = 6xyi + 4yzj + xe^{-y}k$; D the region bounded by the three coordinate planes and the plane $x+y+z = 1$

Surface:
$$ S = S_1\cup S_2\cup S_3\cup S_4 $$
$$ S_1 = \{(x,y,0)/0\leq x\leq 1, 0\leq y\leq 1-x\} $$
$$ S_2 = \{(x,0,z)/0\leq x\leq 1, 0\leq z\leq 1-x\} $$
$$ S_3 = \{(0,y,z)/0\leq y\leq 1, 0\leq z\leq 1-y\} $$
$$ S_4 = \{(x,y,z)/z = 1-x-y, 0\leq x\leq 1, 0\leq y\leq 1-x\} $$
$$ n_1=-k\quad n_2 = -j\quad n_3=-i\quad n_4 = \frac{i+j+k}{\sqrt{3}} $$
$$ \iint_S (F\cdot n)dS = \iint_{S_1} (F\cdot n)dS + \iint_{S_2} (F\cdot n)dS + \iint_{S_3} (F\cdot n)dS + \iint_{S_4} (F\cdot n)dS $$
$$  \iint_S (F\cdot n)dS = \iint_{S_1} (-xe^{-y})dS + \iint_{S_2} (-4yz)dS + \iint_{S_3} (-6xy)dS + \iint_{S_4} \frac1{\sqrt 3}(6xy+4yz+xe^{-y})dS  $$
$$ \iint_S (F\cdot n)dS = \int_0^1\int_0^{1-x}(4y+2xy-4y^2)dydx $$
$$ \iint_S (F\cdot n)dS = \int_1^1(2y^2+xy^2-\frac{4y^3}{3})|_0^{1-x}dx $$
$$  \iint_S (F\cdot n)dS = \int_0^1(3(1-x)^2-\frac73(1-x)^3)dx $$
$$  \iint_S (F\cdot n)dS = ((x-1)^3 + \frac7{12}(x-1)^4)|_0^1 $$
$$ \iint_S(F\cdot n)dS = \frac5{12} $$
Solid:
$$ D = \{(x,y,z)/0\leq x\leq 1, 0\leq y\leq 1-x, 0\leq z\leq 1-x-y\} $$
$$ \nabla \cdot F = \frac{\partial F_1}{\partial x} + \frac{\partial F_2}{\partial y} + \frac{\partial F_3}{\partial z} $$
$$ = 6y + 4z + 0 $$
$$ \iiint_D(\nabla\cdot F)dV = \int_0^1\int_0^{1-x}\int_0^{1-x-y}(6y+4z)dzdydx $$
$$ = \int_0^1\int_0^{1-x}(6yz+2z^2)|_0^{1-x-y}dydx $$
$$ = 2\int_0^1\int_0^{1-x}(1-x-y)(2y-x+1)dydx $$
$$ = 2\int_0^1\int_0^{1-x}(-2y^2+(1-x)y + (1-x)^2)dydx $$
$$ = 2\int_0^1(-\frac{2y^3}3 + \frac{(1-x)y^2}2 + (1-x)^2y)|_0^{1-x} $$
$$ = -\frac53\int_0^1(x-1)^3dx $$
$$ = -\frac5{12}(x-1)^4|_0^1 $$
$$ =\frac5{12} $$
$\therefore$ verified
