1. $y''+3y'+2y=6$
homogenous soln.
$y_c = e^{rx}$
$$ r^2+3r+2=0 $$
$r_1 = -2$
$r_2 = -1$
$$ y_c(x) = C_1e^{-2x}+C_2e^{-x} $$
Rest of It
$$ y_p(x) = A_2x^2+A_1x+A_0 $$
$$ y_p'(x) = 2A_2x+A_1 $$
$$ y_p''(x) = 2A_2 $$
$$ 2A_2+6A_2x+3A_1+2A_2x^2+2A_1x+2A_0 $$
$$ (2A_2)x^2+(6A_2+2A_1)x+(2A_2+3A_1+2A_0)=6 $$
$A_2 = 0$
$A_1 = 0$
$A_0=3$
$$ y(x) = C_1e^{-2x}+C_2e^{-x}+3 $$
3. $y''-10y'+25y=30x+3$
Homo. soln.
$$ r^2-10r+25=0 $$
$$ (x-5)^2=0 $$
$r_1 = r_2 = 5$
$$ y_c = C_1e^{5x}+C_2xe^{5x} $$
 Other Part
 $$ y_p = A_2x^2+A_1x+A_0 $$
 $$ y_p' = 2A_2x+A_1 $$
 $$ y_p'' = 2A_2 $$
Sub into $y''-10y'+25y$
$$ 2A_2 - 20A_2x-10A_1+25A_2x^2+25A_1x+25A_0 $$
$$ (25A_2)x^2 + (25A_1-20A_2)x+(2A_2-10A_1+25A_0) = 30x+3 $$
$A_2 = 0$
$A_1 = \frac{30}{25} = \frac{6}{5}$
$A_0 = \frac{15}{25} = \frac35$
$$ y(x) = C_1e^{5x}+C_2xe^{5x} + \frac65x+\frac35 $$
5. $\frac14y''+y'+y=x^2-2x$
$$ y'' + 4y' + 4y = 4x^2-8x $$
$r_1 = 2$
$r_2 = 2$
$$ y_c(x) = C_1e^{2x}+C_2xe^{2x} $$
$$ y_p(x) = A_2x^2 + A_1x+A_0 $$
$$y_p'(x) = 2A_2x + A_1$$
$$ y_p''(x) = 2A_2 $$
$$ y_p(x) = 2A_2 + 8A_2x+4A_1+4A_2x^2+4A_1x+4A_0 $$
$$ y_p(x) = (4A_2)x^2 + (8A_2+4A_1)x + (4A_2+4A_1+4A_0)=4x^2-8x $$
$A_2 = 1$
$A_1 = -4$
$A_0 = 3$
$$ y(x) = C_1e^{2x}+C_2xe^{2x} + \frac14x^2 - x + \frac34 $$
7. $y''+3y = -48x^2e^{3x}$
$$ r^2 + 3 = 0 $$
$r = \sqrt 3i$
$$ y_c = C_1\cos(\sqrt3x)+C_2\sin(\sqrt3x) $$
$$ y_p = (Ax^2+Bx+C)e^{3x} $$
$$ y_p' = (2Ax+B)e^{3x} + 3(Ax^2+Bx+C)e^{3x} $$
$$ y_p'' = (2A)e^{3x} + 3e^{3x}(2Ax+B) + 3(2Ax+B)e^{3x}+9e^{3x}(Ax^2+Bx+C) $$
9. $y''-y' = -3$
$$ r^2-r = 0 $$
$$ r(r-1) $$
$r_1 = 0$
$r_2 = 1$
$$ y_c = C_1+C_2e^x $$
$y_p = A_1x$
$y_p' = A_0$
$y_p'' = 0$

11. $y''-y'+\frac14y = 3+e^{\frac x2}$
$$ r^2-r+\frac14r = 0 $$
$r_1 = \frac12$
$r_2 = \frac12$
$$ y_c = C_1e^{\frac12x} + C_2xe^{\frac x2} $$
$$ y_p = A_1 + A_0x^2e^{\frac x2} $$
$$ y_p' =  $$
