1. $y' - 3y = \delta(t-2)\qquad y(0) = 0$
$$ L[y']-3L[y] = e^{-2s} $$
$$ sL[y] - 3L[y] = e^{-2s} $$
$$ L[y] = \frac{e^{-2s}}{(s-3)} $$
$$ y = \mathcal U(t-2)e^{3(t-2)} $$
3. $y'' + y = \delta(t-2\pi) \qquad y(0) = 0\quad y'(0)=1$
$$ L[y'']+L[y] = e^{-2\pi s} $$
$$ s^2L[y]-1+L[y] = e^{-2\pi s} $$
$$ L[y] = \frac{e^{-2\pi s}}{(s^2+1)} + \frac1{(s^2+1)} $$
$$ y = \mathcal U(t-2\pi)\sin(t-2\pi) + \sin(t) $$
5. $y'' + y = \delta(t-\frac{\pi}2) + \delta(t-\frac{3\pi}{2})\qquad y(0) = 0\quad y'(0)=0$
$$ L[y''] + L[y] = e^{-\frac{\pi}2s} + e^{-\frac{3\pi}2s} $$
$$ s^2L[y] + L[y] =  $$
$$ L[y] = \frac{e^{-\frac{\pi}2s}}{(s^2+1)} + \frac{e^{-\frac{3\pi}2s}}{(s^2+1)} $$
$$ y = \mathcal U(t-\frac{\pi}2)\sin(t-\frac{\pi}{2}) + \mathcal U(t-\frac{3\pi}2)\sin(t-\frac{3\pi}2) $$

