$$ F = xy\cdot e^{(x-y)} \quad (5,5) $$
$$ \nabla F = [e^{(x-y)}\cdot y + xy\cdot e^{(x-y)}]\hat i + [x\cdot e^{x-y} - xy\cdot e^{x-y}]\hat j $$
$$ = e^{(x-y)}(y+xy)\hat i + e^{(x-y)}(x-xy)\hat j $$
$$ = 30\hat i -20\hat j $$
b. 
$$ F = x^2y\hat i + xy^2\hat j + 2xyz\hat k $$
$$ \nabla \times F = (\frac{\partial F_z}{\partial y} - \frac{\partial F_y}{\partial z})\hat i - (\frac{\partial F_z}{\partial x} - \frac{\partial F_x}{\partial z})\hat j + (\frac{\partial F_y}{\partial x} - \frac{\partial F_x}{\partial y})\hat k $$
$$ = (2xz)\hat i - (2yz)\hat j + (y^2 - x^2)\hat k $$
$$ \nabla\cdot \uparrow\; = 2z - 2z + 0 = 0 $$
2. a
$$ F = (5x + 4y)\hat i + (4x - 8y^3)\hat j $$
$$ 4 = 4 $$
$$ \int(5x + 4y)dx = \frac52x^2 + 4xy + g(y) $$
$$ \frac{\partial }{\partial y}(\frac{5}{2}x^2 + 4xy + g(y)) = 4x + g'(y) $$
$g'(y) = -8y^3$
$g(y) = -2y^4$
$$ \phi = \frac{5}{2}x^2 + 4xy - 2y^4 $$
$$ \phi(0,0) - \phi(-1,1) = 0 - \frac{5}{2} + 4 + 2 = \frac{7}{2}$$
c.

$$ y = -x $$
$$ dy = -1dx $$
$$ \int_{1}^{0} (5x + 4y)dx + (4x - 8y^3)dy = \int_{1}^{0}(5x - 4x)dx - (4x + 8x^3)dx $$
$$ \int_{1}^{0}(-3x - 8x^3)dx $$
$$ -\frac{3}{2}x^2 - 2x^4 = -\frac{7}{2} $$
3
$$ \oint(-xy^2dx + x^2y\;dy) =  $$

$$ = 30xy\hat i $$

### 9.5.18
$$ = 2xy^2(2z+1)^2\hat i + 2x^2y(2z+1)^2\hat j + 4x^2y^2(2z+1)\hat k $$

$$ \frac12x^2 + 2xy + g(y) $$
$$ 2x + g'(y) $$