## NMM2270.2.4
2.4: 1-37(odd)

#### Uses:
- [[Exact Differential Equation]]

1. $(2x-1)dx + (3y+7)dy = 0$
$M(x,y) = (2x-1)$
$N(x,y) = (3y+7)$
$$ \frac{\partial}{\partial y} (2x-1) = \frac{\partial}{\partial x}(3y+7) $$
$$ 0 = 0 $$
$\therefore$ Exact
$$ \frac{\partial}{\partial x}f = (2x-1) $$
$$ \int\frac{\partial}{\partial x}f\;dx = \int(2x-1)dx $$
$$ f(x,y) = x^2 - x + g(y) $$
Next Step:
$$ \frac{\partial}{\partial y}f = N $$
$$ \frac{\partial f}{\partial y} = (3y + 7) $$
$$ \frac{\partial}{\partial y}(x^2-x+g(y)) = 3y+7 $$
$$ g'(y) = 3y+7 $$
$$ \int\frac{d}{dy}g(y)dy = \int(3y+7)dy $$
$$ g(y) = \frac32y^2 + 7y + D $$
$\therefore f(x,y)= x^2-x+\frac32y^2+7y+D$
- We know solution is $f(x,y) = c$ so:
$$ f(x,y) = c $$
$$ x^2-x+\frac32y^2+7y+D = C $$
let $B = C-D$
$$ y(\frac32y + 7) = B-x^2+x $$
Usually solve for y pretty sure

3. $(5x+4y)dx + (4x-8y^3)dy = 0$
$M(x,y) = (5x+4y)$
$N(x,y)=(4x-8y^3)$
$$ \frac{\partial M}{\partial y} = \frac{\partial N}{\partial x} $$
$$ \frac{\partial}{\partial y}(5x+4y) = \frac{\partial}{\partial x}(4x-8y^3) $$
$$ 4 = 4 $$
$\therefore$ exact
$$ \int\frac{\partial f}{\partial x}dx = \int(5x + 4y)dx $$
$$ f(x,y) = \frac52x^2 + 4yx + g(y) $$
Next Part:
$$ \frac{\partial f}{\partial y} = N $$
$$ \frac{\partial}{\partial y}(\frac52x^2 + 4yx + g(y)) = (4x-8y^3) $$
$$ 4x + g'(y) = 4x - 8y^3 $$
$$ \int\frac{d}{dy}g(y)dy = -8\int y^3dy $$
$$ g(y) = -\frac{8}{4}y^4 $$
$$ f(x,y) = \frac52x^2+4yx-2y^4 + D $$
$$ c = \frac52x^2 + 4yx - 2y^4 $$
5. $(2xy^2-3)dx + (2x^2y+4)dy = 0$
$M(x,y) = (2xy^2-3)$
$N(x,y) = (2x^2y+4)$
$$ \frac{\partial M}{\partial y} = \frac{\partial N}{\partial x} $$
$$ \frac{\partial}{\partial y}(2xy^2-3) = \frac{\partial}{\partial x}(2x^2y+4) $$
$$ 4xy = 4xy $$
$\therefore$ Exact
$$ \int\frac{\partial f}{\partial x}dx = \int(2xy^2-3)dx $$
$$ f(x,y) = x^2y^2-3x + g(y) $$
Next Part
$$ \frac{df}{dy} = (2x^2y+4) $$
$$ \frac{d}{dy}(x^2y^2-3x+g(y)) = 2x^2y+4 $$
$$ \cancel{2x^2y} + g'(y) = \cancel{2x^2y}+4 $$
$$ \int g'(y)dy = \int4dy $$
$$ g(y) = 4y + D $$
$$ f(x,y) = x^2y^2-3x+4y+D $$
$$ c = x^2y^2-3x+4y $$
7. $(x^2-y^2)dx + (x^2-2xy)dy = 0$
$M(x,y) = (x^2-y^2)$
$N(x,y) = (x^2-2xy)$
$$ \frac{\partial M}{\partial y} = \frac{\partial N}{\partial x} $$
$$ \frac{\partial}{\partial y}(x^2-y^2) = \frac{\partial}{\partial x}(x^2-2xy) $$
$$ -2y = 2x-2y $$
$\therefore$ not Exact

9. $(x-y^3+y^2\sin x)dx = (3xy^2 +2y\cos x)dy$
$$ (x-y^3+y^2\sin x)dx - (3xy^2+2y\cos x)dy = 0 $$
$M(x,y) = (x-y^3+y^2\sin x)$
$N(x,y) = (-3xy^2-2y\cos x)$
$$ \frac{\partial M}{\partial y} = \frac{\partial N}{\partial x} $$
$$ -3y^2+2y\sin x = -3y^2 +2y\sin x  $$
$\therefore$ Exact
$$ \int\frac{df}{dx}dx = \int(x-y^3+y^2\sin x)dx $$
$$ f(x,y) = \frac12x^2-xy^3-y^2\cos x + g(y) $$
$$ \frac{\partial f}{\partial y} = (-3xy^2-2y\cos x) $$
$$ -3xy^2-2y\cos x + g'(y) = (-2xy^2-2y\cos x) $$
$$ \int g'(y)dy = \int xy^2dy $$
$$ g(y) = \frac13xy^3 $$
$$ f(x,y) = \frac12x^2-xy^3-y^2\cos x + \frac13y^3 = c $$
```ad-attention
check where i went wrong. should be missing the $\frac13y^3$
```
11. $(y\ln y - e^{-xy}) dx + (\frac1y+x\ln y)dy = 0$
$M(x,y) = (y\ln y - e^{-xy})$
$N(x,y) = (\frac1y + x\ln y)$
$$ \frac{\partial M}{\partial y} = \frac{\partial N}{\partial x} $$
$$ \frac{\partial}{\partial y}(y\ln y - e^{-xy}) = \frac{\partial}{\partial x}(\frac1y + x\ln y) $$
$$ \ln y + 1 + xe^{-xy}=\ln y $$
$\therefore$ not exact

13. $x\frac{dy}{dx} = 2xe^x-y+6x^2$
$$ xdy + (-2xe^x + y - 6x^2)dx = 0 $$
$M(x,y) = (-2xe^x + y - 6x^2)$
$N(x,y) = (x)$
$$ \frac{\partial M}{\partial y} = \frac{\partial N}{\partial x} $$
$$ \frac{\partial}{\partial y}(-2xe^x + y - 6x^2) = \frac{\partial}{\partial x} x $$
$$ 1 = 1 $$
$\therefore$ exact

$$ \int\frac{\partial f}{\partial x}dx = \int(-2xe^x + y -6x^2)dx $$
$$ f(x,y) = -2\int(xe^x)dx + xy - 2x^3 $$
[[Integration by Parts]]
$dv = e^xdx\qquad v = e^x$
$u = x\qquad du = dx$
$$ \int u\cdot dv = u\cdot v - \int v\cdot du $$
$$ \int xe^x = xe^x - \int e^xdx $$
$$ = xe^x - e^x $$
Sub in
$$ f(x,y) = -2xe^x + 2e^x + xy - 2x^3 + g(y) $$
Next Part
$$ \frac{\partial f}{\partial y} = x $$
$$ \frac{\partial}{\partial y}(2xe^x - 2e^x + xy - 2x^3 + g(y)) = x $$
$$ x + g'(y) = x $$
$$ \int g'(y) = \int0 $$
$$ g(y) = D $$
$$ f(x,y) = -2xe^x + 2e^x + xy - 2x^3 + D = c $$
15. $(x^2y^3 - \frac1{1+9x^2})\frac{dx}{dy}+x^3y^2 = 0$
$$ (x^2y^3-\frac1{1+9x^2})dx + (x^3y^2)dy = 0 $$
$M(x,y) = (x^2y^3 - \frac1{1+9x^2})$
$N(x,y) = (x^3y^2)$
$$ \frac{\partial M}{\partial y} = \frac{\partial N}{\partial x} $$
$$ \frac{\partial}{\partial y}(x^2y^3 - \frac1{1+9x^2}) = \frac{\partial}{\partial x} (x^3y^2) $$
$$ 3x^2y^2 = 3x^2y^2 $$
$\therefore$ exact
$$ \int \frac{\partial f}{\partial x}dx = \int(x^2y^3 - \frac1{1+9x^2})dx $$
$$ f(x,y) = \frac13x^3y^3 - \frac13\tan^{-1}(3x) + g(y) $$
$$ \frac{\partial f}{\partial y} = x^3y^2 $$
$$ \frac{\partial}{\partial y}(x^3y^3 - \tan^{-1}(3x) + g(y)) = x^3y^2 $$
$$ x^3y^2 + g'(y) = x^3y^2 $$
$$ \int g'(y) = \int 0 $$
$$ g(y) = D $$
$$ f(x,y) = x^3y^3-\tan^{-1}(3x) + D $$
17. $(\tan x - \sin x\sin y)dx + (\cos x\cos y)dy = 0$
$M(x,y) = (\tan x-\sin x\sin y)$
$N(x,y) = (\cos x\cos y)$
$$ \frac{\partial M}{\partial y} = \frac{\partial N}{\partial x} $$
$$ \frac{\partial}{\partial y}(\tan x - \sin x\sin y) = \frac{\partial}{\partial x}(\cos x\cos y) $$
$$ -\sin x\cos y = -\sin x\cos y $$
$\therefore$ Exact
$$ \int\frac{df}{dx}dx = \int (\tan x - \sin x\sin y)dx $$
$$ f(x,y) = -\ln|\cos x| + \cos x\sin y + g(y) $$
$$ \frac{\partial f}{\partial y} = (\cos x\cos y) $$
$$ \frac{\partial}{\partial y}(-\ln|\cos x| + \cos x\sin y + g(y)) = (\cos x\cos y) $$
$$ \cos x\cos y + g'(y) = \cos x\cos y $$
$$ \int g'(y) = \int 0 $$
$$ g(y) = D $$
$$ f(x,y) = -\ln|\cos x| + \cos x\sin y + D $$
19. $(4t^3y - 15t^2-y)dt + (t^4+3y^2-t)dy = 0$
$M(t,y) = (4t^3y - 15t^2 - y)$
$N(t,y) = (t^4+3y^2-t)$
$$ \frac{\partial M}{\partial y} = \frac{\partial N}{\partial t} $$
$$ \frac{\partial}{\partial y}(4t^3y-15t^2-y) = \frac{\partial}{\partial t}(t^4+3y^2-t) $$
$$ 4t^3 - 1 = 4t^3 - 1 $$
$\therefore$ Exact
$$ \int\frac{\partial f}{\partial t} = \int(4t^3y - 15t^2-y)dt $$
$$ f(t,y) = t^4y - 5t^3 - ty + g(y) $$
$$ \frac{\partial f}{\partial y} = (t^4+3y^2-t) $$
$$ \frac{\partial}{\partial y}(t^4y-5t^3-ty+g(y)) = (t^4+3y^2-t) $$
$$ t^4-t+g'(y) = t^4+3y^2-t $$
$$ \int g'(y) = \int3y^2 $$
$$ g(y) = y^3 $$
$$ f(x,y) = t^4y-5t^3-ty+y^3+D $$
21. $(x+y)^2dx + (2xy+x^2-1)dy = 0$,  y(1) = 1
$M(x,y) = (x+y)^2 = x^2 + 2xy + y^2$
$N(x,y) = (2xy+x^2-1)$
$$ \frac{\partial M}{\partial y} = \frac{\partial N}{\partial x} $$
$$ \frac{\partial}{\partial y}(x+y)^2 = \frac{\partial}{\partial x}(2xy + x^2-1) $$
$$ 2(x+y) \cdot 1 = 2y+2x $$
$\therefore$ Exact
$$ \int\frac{\partial f}{\partial x} = \int(x^2+2xy+y^2)dx $$
$$ f(x,y) = \frac13x^3 + x^2y + xy^2 + g(y) $$
$$ \frac{\partial f}{\partial y} = (2xy + x^2 - 1) $$
$$ \frac{\partial}{\partial y}(\frac13x^3+x^2y+xy^2+g(y)) = 2xy+x^2-1 $$
$$ x^2+2xy+g'(y) = 2xy+x^2-1 $$
$$ \int g'(y) = \int-1 $$
$$ g(y) = -y $$
$$ f(x,y) = \frac13x^3+x^2y+xy^2-y+D = 0 $$
$$ \frac13(1)^3 + (1)^2(1) + (1)(1)^2-(1) + D = 0 $$
$$ \frac13 + 1 + 1 - 1 + D = 0 $$
$$ D = -\frac43 $$
$$  \frac13x^3+x^2y+xy^2-y-\frac43 = 0 $$
23. $(4y+2t-5)dt + (6y+4t-1)dy = 0$, $y(-1)=2$
$M = (4y+2t-5)$
$N = (6y+4t-1)$
$$ \frac{\partial M}{\partial y} = \frac{\partial N}{\partial t} $$
$$ 4 = 4 $$
$\therefore$ Exact
$$ \int \frac{\partial f}{\partial t}dt = \int(2y+2t-5)dt $$
$$ f = 2yt+t^2-5t + g(y) $$
$$ \frac{\partial f}{\partial y} = 6y+4t-1 $$
$$ \frac{\partial}{\partial y}(2yt+t^2-5t+g(y)) = 6y+4t-1 $$
$$ 2t+g'(y) = 6y+4t-1 $$
$$ \int g'(y) = \int(6y+2t-1) $$
$$ g(y) = 3y^2+2ty-y+C $$
$$ f = 2yt+t^2-5t+3y^2+2ty-y+C = c $$
$$ f = 4yt + t^2+3y^2-5t-y+C = c $$
$$ 4(2)(-1)+(-1)^2 + 3(2)^2-5(-1)-(2)=C_1 $$
$$ -8 + 1+12+5-2 = 8 = C_1 $$
$$ f = 4yt+t^2+3y^2-5t-y=8 $$
