1. $\frac{dx}{dt} = -x + y$
$\frac{dy}{dt} = 2x$
$x(0) = 0, \quad y(0) = 1$
$$ L[x'] = -L[x] + L[y] $$
$$ sX(s)+X(s) = Y(s) $$

$$ L[\frac{dy}{dt}] = 2L[x] $$
$$ sY(s) - 1 = 2X(s) $$
$$ s^2X(s) + sX(s) - 1 = 2X(s) $$
$$ s^2X(s) + sX(s) - 2X(s) = 1 $$
$$ X(s)(s^2 + s - 2) = 1 $$
$$ L^{-1}[X(s)] = \frac{1}{(s^2 + s -2)} = \frac{1}{(s+2)(s-1)} $$

$\frac{1}{(s+2)(s-1)} = \frac{A}{(s+2)} + \frac{B}{(s-1)}$
$1= As - A + Bs +2B$
$1 = (2B-A) + (A+B)s$

$A = -\frac13$
$B = \frac13$

$$ x(s) = -\frac1{3(s+2)} + \frac1{3(s-1)} $$
$$ x(t) = -\frac13e^{-2t} + \frac13e^{t} $$

$$ Y(s) = \frac{2}{s(s+2)(s-1)} + \frac1s $$
$\frac{2}{s(s+2)(s-1)} = \frac{A}{s} + \frac{B}{(s+2)} + \frac{C}{(s-1)}$
$2 = (A+B+C)s^2 + (A-B+2C)s - 2A$

$0 = (-1)+B+C$
$0 = (-1)-B + 2C$
$A = -1$
$B = \frac13$
$C = \frac23$

$$ Y(s) = \frac1{3(s+2)} + \frac{2}{3(s-1)} $$
3. $\frac{dx}{dt} = x-2y$
$\frac{dy}{dt} = 5x-y$
$x(0) = -1, \quad y(0) = 2$
$$ L[x'] = X(s) - 2Y(s) $$
$$ sX(s) +1 = X(s) - 2Y(s) $$
$$ -\frac{sX(s)}{2} + \frac{X(s)}2 - \frac12 = Y(s) $$
$$ L[y'] = 5X(s) - Y(s) $$
$$ sY(s) - 2 = 5X(s) - Y(s) $$
$$ sY(s) + Y(s) = 5X(s) + 2 $$
$$ Y(s) = \frac{5X(s)}{(s+1)} + \frac{2}{(s+1)} $$

$$ -sX(s) + X(s) - 1 = \frac{10X(s)}{(s+1)} + \frac4{(s+1)} $$
$$ -sX(s) + X(s) - \frac{10X(s)}{s+1} = \frac4{(s+1)} + 1 $$
$$ -s(s+1)X(s) + (s+1)X(s) - 10X(s) = 4 + s + 1 $$
$$ X(s)(-s^2 - s+s+1-10) = 4+s+1 $$
$$ X(s)(-s^2-9) = 4+s+1 $$
$$ X(s) = \frac{-4}{(s^2+9)} + \frac{-s}{(s^2+9)} + \frac{-1}{(s^2+9)} $$
$$ x(t) = \frac{-4}{3}\sin(3t) - \cos(3t) -\frac13 \sin(3t) $$

$$ Y(s) = \frac{5}{(s+1)}(\frac{-4}{(s^2+9)} + \frac{-s}{(s^2+9)} + \frac{-1}{(s^2+9)}) + \frac{2}{(s+1)} $$
$$ Y(s) = \frac{-20}{(s^3 +s^2 + 9s + 9)} + \frac{-5s}{(s^3 +s^2 + 9s + 9)} + \frac{-5}{(s^3 +s^2 + 9s + 9)} + \frac{2}{(s+1)} $$
$$ Y(s) = \frac{-20}{(x+1)(x^2+9)} - \frac{5s}{(x+1)(x^2+9)} - \frac{5}{(x+1)(x^2+9)} + \frac2{(s+1)} $$




