## NMM 2270 2.3 PPs
Uses: [[Linear 1st Order ODE]]
1. $\frac{dy}{dx} = 5y$
$$ \frac{dy}{dx} - 5y = 0 $$
$$ y(x) = e^{+5x}\cdot\int e^{-5x}\cdot 0 dx + C\cdot e^{-5x}$$
$$ y(x) = C\cdot e^{5x} $$
3. $\frac{dy}{dx} + y = e^{3x}$
$$ y(x) = e^{-x}\cdot\int e^x \cdot e^{3x}dx + C\cdot e^{-x} $$
$$ y(x) = e^{-x}\cdot\int e^{4x}dx + C\cdot e^{-x} $$
$$ y(x) = \frac14e^{3x} + C\cdot e^{-x} $$
5. $y' + 3x^2y = x^2$
$$ y(x) = e^{-x^3}\cdot\int e^{x^3}x^2 dx + C\cdot e^{-x^3} $$
$$ y(x) = \frac13e^{-x^3}\cdot e^{x^3} + C\cdot e^{-x^3} $$
$$ \frac13 + C\cdot e^{-x^3} $$
7. $x^2 y' + xy = 1$
$$ y' + \frac1xy = \frac1{x^2} $$
$$ y(x) = e^{-\ln|x|}\cdot\int e^{\ln|x|}\frac1{x^2} + C\cdot e^{-\ln|x|} $$
$$ y(x) = \frac{1}{x}\cdot\int \frac{1}{x} + C\cdot \frac{1}{x} $$
$$ \frac{1}{x} \cdot \ln{x}+C\cdot\frac1{x} $$
9. $\frac{xdy}{dx} - y = x^2\sin x$
$$ \frac{dy}{dx} - \frac{1}{x}y = x\sin x $$
$$ y(x) = e^{\ln x}\cdot\int e^{-\ln x}x\sin x + C\cdot e^{\ln x} $$
$$ y(x) = x\cdot\int\frac{1}{x}x\sin x + C\cdot x$$
$$ y(x) = x\cdot\int\sin x + C\cdot x $$
$$ y(x) = -x\cdot\cos x + C\cdot x $$
11. $x\frac{dy}{dx} + 4y = x^3 - x$
$$ \frac{dy}{dx} + \frac{4y}{x} = x^2-1 $$
$$ y(x) = e^{-4\ln x}\cdot\int e^{4\ln x}\cdot(x^2 - 1) + C\cdot e^{-4\ln x} $$
$$ y(x) = x^{-4}\cdot\int x^4\cdot(x^2 - 1) + C\cdot x^{-4} $$
$$ y(x) = x^{-4}\cdot(\int x^6 -\int x^4) + C\cdot x^{-4} $$
$$ x^{-4}\cdot(\frac17x^7 - \frac15x^5) + C\cdot x^{-4} $$
$$ \frac17x^3 - \frac15x + C\cdot x^{-4} $$
13. $x^2y' + x(x+2)y = e^x$
$$ y' + \frac{x+2}{x}y = \frac{e^x}{x^2} $$
$$ y' + 2(\frac12+\frac1x)y = \frac{e^x}{x^2} $$
$$ y(x) = e^{-x-2\ln x}\cdot\int e^{x+2\ln x}\cdot \frac{e^x}{x^2}\cdot dx + C\cdot e^{-x-2\ln x} $$
$$ y(x) = e^{-x}e^{\ln x^{-2}}\cdot\int e^{x}\cdot x^2\cdot\frac{e^x}{x^2}\cdot dx + C\cdot e^{-x}\cdot e^{\ln x^{-2}} $$
$$ y(x) = e^{-x}x^{-2}\cdot\int e^{2x} + C\cdot e^{-x}\cdot x^{-2} $$
$$ y(x) = e^{-x}x^{-2}\cdot\frac12e^{2x} + C\cdot e^{-x}\cdot x^{-2} $$
$$ y(x) = \frac12e^xx^{-2} + Ce^{-x}x^{-2} $$
15. $ydx - 4(x+y^6)dy = 0$
$$ \frac{dx}{dy} - \frac{4x}{y} - 4y^5 = 0 $$
$\mu(y) = -4\ln y$
$q(y) = 4y^5$
$$ x(y) = e^{\ln y^4}\cdot\int e^{\ln y^{-4}}\cdot4y^5dy + C\cdot e^{\ln y^4} $$
$$ x(y) = y^4\cdot\int y^{-4}\cdot4y^5dy + C\cdot y^4 $$
$$ x(y) = y^4\cdot\int 4ydy + C\cdot y^4 $$
$$ x(y) = 2\cdot y^4\cdot y^2 + C\cdot y^4 $$
$$ x(y) = y^4(2y^2 + C) $$
17. $\cos x\frac{dy}{dx} + (\sin x)y = 1$
$$ \frac{dy}{dx} +\frac{\sin x}{\cos x}y = \frac1{\cos x} $$
$$ \frac{dy}{dx} + \tan x\cdot y = \sec x $$
$\mu(x) = -\ln|\cos x|$
$$ y(x) = e^{\ln|\cos x|}\cdot\int e^{\ln|\cos x|^{-1}}\cdot\sec x + C\cdot e^{\ln|\cos x|} $$
$$ y(x) = \cos x\cdot\int\frac1{\cos x}\cdot\sec x + C\cdot\cos x $$
$$ y(x) = \cos x\cdot\int\sec^2x + C\cdot\cos x $$
$$ y(x) = \cos x\cdot\tan x  + C\cdot\cos x$$
$$ y(x) = \sin x + C\cdot\cos x $$
19. $(x+1)\frac{dy}{dx} + (x+2)y = 2xe^{-x}$
$$ \frac{dy}{dx} + \frac{x+2}{x+1}y = \frac{2xe^{-x}}{x+1} $$
```ad-question
```

21. $\frac{dr}{d\theta} + r\sec\theta = \cos\theta$
$\mu(\theta) = \ln|\sec\theta + \tan\theta|$
$$ r(\theta) = \frac1{\sec\theta + \tan\theta}\cdot\int(\cos\theta\sec\theta + \cos\theta\tan\theta)d\theta + \frac{C}{\sec\theta + \tan\theta} $$
$$ r(\theta) = \frac1{\sec\theta + \tan\theta}\cdot(\int\cos\theta\sec\theta d\theta + \int\cos\theta\tan\theta d\theta) + \frac{C}{\sec\theta + \tan\theta} $$
$$ r(\theta) = \frac1{\frac1{\cos\theta} + \frac{\sin\theta}{\cos\theta}}\cdot(\theta -\cos\theta) + \frac{C}{\frac1{\cos\theta} + \frac{\sin\theta}{\cos\theta}} $$
$$ r(\theta) = \frac{\cos\theta}{1 + \sin\theta}\cdot(\theta-\cos\theta) + \frac{C\cos\theta}{1 + \sin\theta} $$
23. 