### 9.12 #3
$\oint_C -y^2dx + x^2 dy = \iint_R (2x+2y) dA$ where C is the circle $x = 3\cos t$, $y = 3\sin t$, $0\leq t\leq 2\pi$

#### Green's Theorem:
$y = 3\sin t\qquad dy = 3\cos t dt$
$x = 3\cos t\qquad dx = 3\sin t dt$
$$ \oint_C -y^2dx + x^2 dy = \int_0^{2\pi}-(3\sin t)^2 \cdot -3\sin t dt + (3\cos t)^2\cdot 3\cos t $$
$$ = \int_0^{2\pi} 27\sin^3t dt + 27\cos^3 t dt $$
$$ = 27\int_0^{2\pi} (1-\cos^2t)(\sin t)dt + 27\int_0^{2\pi}(1-\sin^2 t)(\cos t)dt $$
U Sub:
$$ u = \cos t \qquad \qquad u = \sin t $$
$$ du = -\sin t \qquad\qquad du = \cos t $$
$$ \int_0^{2\pi} (1-\cos^2 t)(\sin t)dt = -\int (1-u^2)du \qquad\qquad \int_0^{2\pi}(1-\sin^2 t)(\cos t)dt = -\int (1-u^2)du $$
$$ = -(u - \frac13u^3) \qquad\qquad\qquad = u-\frac13 u^3 $$
$$ = 27(-\cos t + \frac13\cos^3 t + \sin t - \frac13\sin^3t)|_0^{2\pi} $$
$$ = 27[(-1+\frac13 + 0 - 0) - (-1 + \frac13 + 0 - 0)] $$
$$ = 27[0] $$
$$ = 0 $$
#### Double Integral:
$$ \iint_R(2x + 2y)dA = \iint_R (2\cos\theta + 2\sin\theta) r\;dr\;d\theta $$
$$ = \int_0^{2\pi}\int_0^3 2r^2(\cos\theta + \sin\theta)dr\;d\theta $$
$$ = \int_0^{2\pi}[\frac23r^3]_0^3(\cos\theta + \sin\theta) \; d\theta $$
$$ = \int_0^{2\pi}[18 - 0](\cos\theta+\sin\theta)\;d\theta $$
$$ = 18\int_0^{2\pi}(\cos\theta + \sin\theta)d\theta $$
$$ = 18(\sin\theta-\cos\theta)|_0^{2\pi} $$
$$ = 18[(0-1) - (0-1)] $$
$$ = 18[0] $$
$$ = 0 $$

$$ \oint_C -y^2dx + x^2 dy = \iint_R (2x+2y) dA $$
$$ 0 = 0 $$
$\therefore$ The theorem is validated
