Find Laplace Transformations for the Following
1. $f(t) = \begin{cases} -1,\; 0\leq t < 1 \\ 1, \qquad\;\; t\geq 1\end{cases}$
$$ \mathcal L[f(t)] = \int_0^1e^{-st}(-1)dt + \int_1^\infty e^{-st}(1) $$
$$ = (\frac{e^{-s(1)}}{s} - \frac{e^{-s(0)}}{s}) + (\frac{-e^{-s(\infty)}}{s} - \frac{-e^{-s(1)}}{s}) $$
$$ = -\frac{1}{s} + \frac{e^{-s}}s + \frac{e^{-s}}s $$
$$ = \frac{2e^{-s}-1}s $$
3. $f(t) = \begin{cases} t,\;\; 0\leq t < 1 \\ 1, \qquad\;\; t\geq 1\end{cases}$
$$ \mathcal L[f(t)] = \int_0^1te^{-st} + \int_1^\infty e^{-st} $$
-------------------- IBP -----------------------
$$ \int te^{-st} $$
$dv = e^{-st} \to v = -\frac{e^{-st}}s$
$u = t\to du = dt$
$$ = t\cdot -\frac{e^{-st}}s + \int -\frac{e^{-st}}s $$
$$ = -\frac{te^{-st}}s + \frac{e^{-st}}{s^2} $$
---------------- IBP End ------------------
$$ = [(\frac{e^{-s(1)}}{s^2} - \frac{te^{-s(1)}}s) - (\frac{e^{-s(0)}}{s^2} - \frac{te^{-s(0)}}s)] + (-\frac{e^{-s(\infty)}}s + \frac{e^{-s(1)}}s) $$
$$ = \frac{e^{-s}}{s^2}-\frac{e^{-s}}s - \frac1{s^2} + \frac{e^{-s}}s  $$
$$ = \frac{e^{-s}-1}{s^2} $$
```ad-note
e^-s should be negative and 1 should be +
```

11. $f(t) = e^{t+7}$
$$ \mathcal L[f(t)] = \int_0^\infty e^te^7e^{-st} $$
$$ = e^7[\int_0^\infty e^{t(1-s)}] $$
$$ = e^7[\frac{e^{(\infty)(1-s)}}{1-s} - \frac{1}{1-s}] $$
$$ = \frac{e^{7}}{1-s} \qquad s > 1 $$
13. $f(t) = te^{4t}$
$$ \mathcal L[f(t)] = \int_0^\infty te^{t(4-s)} $$
-------------- IBP -------------------------------------------------
$dv = e^{t(4-s)}\to v=\frac{e^{t(4-s)}}{4-s}$
$u = t\to du = dt$
$$ = \frac{te^{t(4-s)}}{4-s} - \int \frac{e^{t(4-s)}}{4-s} $$
$$ = \frac{te^{t(4-s)}}{4-s} - \frac{e^{t(4-s)}}{(4-s)^2} $$
-------------------------- END -----------------------------------
$$ [(\frac{(\infty)e^{(\infty)(4-s)}}{4-s} - \frac{e^{(\infty)(4-s)}}{(4-s)^2}) - (\frac{(0)e^{(0)(4-s)}}{4-s} - \frac{e^{(0)(4-s)}}{(4-s)^2})] $$
$$ = \frac{1}{(4-s)^2}\qquad s>4 $$
19. $f(t) = 2t^4$
$$ \mathcal L[f(t)] = 2\frac{4!}{s^5} $$
$$ = \frac{48}{s^5} $$
21. $f(t) = 4t - 10$
$$ \mathcal L[4t] - \mathcal L[10] = \frac{4}{s^2} - \frac{10}s $$
25. $f(t) = (t+1)^3$
$$ f(t) = t^3 + 3t^2+3t+1 $$
do laplace of each

27. $f(t) = 1+e^{4t}$
$$ \mathcal L[1] + \mathcal L[e^{4t}] = \frac1s + \frac1{s-4} $$
