[[NMM2276.Assignment2.Page1]]
[[NMM2276.Assignment2.Page2]]
[[NMM2276.Assignment2.Page3]]
[[NMM2276.Assignment2.Page4]]

#### 9.5 #25
find a vector that gives the direction in which the given function increases most rapidly at the indicated point. Find the maximum rate.

$\therefore$ calculate gradient

$$ F(x,y,z) = x^2 + 4xz + 2yz^2\;;\quad (1,2,-1) $$
$$  \nabla F(x,y,z) = \frac{\partial F}{\partial x}\hat i + \frac{\partial F}{\partial y}\hat j + \frac{\partial F}{\partial z}\hat k  $$

$\frac{\partial F}{\partial x} = 2x + 4z$
$\frac{\partial F}{\partial y} = 2z^2$
$\frac{\partial F}{\partial z} = 4x + 4yz$
$$ \nabla F(x,y,z) = (2x+4z)\hat i + 2z^2\;\hat j + (4x+4yz)\hat k $$
$$ \nabla F(1,2,-1) = (2-4)\hat i + 2\hat j + (4-8)\hat k $$
$$ \nabla F(1,2,-1) = -2\hat i + 2\hat j -4\hat k $$
$$ ||\nabla F(1,2,-1)|| = \sqrt{(-2)^2 + 2^2 + (-4)^2} $$
$$ ||\nabla F(1,2,-1)|| = \sqrt{24} $$
$\therefore$ the vector for the direction where the function increases the most is $\nabla F(1,2,-1) = -2\hat i + 2\hat j -4\hat k$ and the magnitude is $\sqrt {24}$

#### 9.6 #17
find an equation of the tangent plane to the graph of the given equation at the indicated point.
$$ x^2-y^2-3z^2 = 5\;;\quad (6,2,3) $$
##### Equation for [[Tangent Plane]]:
 $$ \frac{\partial }{\partial x}F(x_0, y_0, z_0)(x-x_0) + \frac{\partial }{\partial y}F(x_0, y_0, z_0)(y-y_0)+\frac{\partial }{\partial z}F(x_0, y_0, z_0)(z-z_0)=0 $$
$\frac{\partial F}{\partial x} = 2x$
$\frac{\partial F}{\partial y} = -2y$
$\frac{\partial F}{\partial z} = -6z$

Sub in Points:

$\frac{\partial }{\partial x}F(x_0, y_0, z_0)= 12$
$\frac{\partial }{\partial y}F(x_0, y_0, z_0)= -4$
$\frac{\partial }{\partial z}F(x_0, y_0, z_0)=-18$

Sub in Equations:

$$ 12\cdot (x-6) -4\cdot (y-2)-18\cdot (z-3) = 0 $$
$$ 12x - 72 - 4y + 8 - 18z + 54 = 0 $$
$$ 12x - 4y - 18z = 10 $$
$$ 6x - 2y - 9z = 5 $$
#### 9.7 #13
find the curl and the divergence of the given vector field.
$$ F(x,y,z) = xe^{-z}\hat i + 4yz^2\hat j + 3ye^{-z}\hat k $$
##### [[Curl]]:
$$ \nabla \times\vec F = \hat i(\frac{\partial F_z}{\partial y} - \frac{\partial F_y}{\partial z}) - \hat j(\frac{\partial F_z}{\partial x} - \frac{\partial F_x}{\partial z})+\hat k(\frac{\partial F_y}{\partial x} - \frac{\partial F_x}{\partial y}) $$
$\frac{\partial F_z}{\partial y} = 3e^{-z}$
$\frac{\partial F_y}{\partial z} = 8yz$
$\frac{\partial F_z}{\partial x} = 0$
$\frac{\partial F_x}{\partial z} = -xe^{-z}$
$\frac{\partial F_y}{\partial x} = 0$
$\frac{\partial F_x}{\partial y} = 0$
$$ \nabla \times\vec F = [(3e^{-z}) - (8yz)]\hat i - xe^{-z}\hat j $$

##### [[Divergence]]:
$$  \nabla\cdot\vec F = (\frac{\partial F_x}{\partial x}) + (\frac{\partial F_y}{\partial y})+(\frac{\partial F_z}{\partial z})  $$
$\frac{\partial F_x}{\partial x} = e^{-z}$
$\frac{\partial F_y}{\partial y} = 4z^2$
$\frac{\partial F_z}{\partial z} = -3ye^{-z}$
$$ \nabla \cdot \vec F = e^{-z} + 4z^2 - 3ye^{-z} $$

#### 9.7 #27
verify the given identity. Assume continuity of all partial derivatives.
$$ \nabla \cdot (fF) = f(\nabla \cdot F) + F\cdot \nabla f $$
$$ \nabla \cdot (fF) = (\frac{\partial }{\partial x}\hat i + \frac{\partial }{\partial y}\hat j + \frac{\partial }{\partial z}\hat k)\cdot (fF_x\hat i + fF_y\hat j + fF_z\hat k) $$
$$ = \frac{\partial }{\partial x}(fF_x) + \frac{\partial }{\partial y}(fF_y) + \frac{\partial }{\partial z}(fF_z) $$
$$ = f\frac{\partial F_x}{\partial x} + F_x\frac{\partial f}{\partial x} + f\frac{\partial F_y}{\partial y} + F_y\frac{\partial f}{\partial y} + f\frac{\partial F_z}{\partial z} + F_z\frac{\partial f}{\partial z} $$
$$ = f(\frac{\partial F_x}{\partial x} + \frac{\partial F_y}{\partial y} + \frac{\partial F_z}{\partial z}) + F_x\frac{\partial f}{\partial x} + F_y\frac{\partial f}{\partial y} + F_z\frac{\partial f}{\partial z} $$
$$ \nabla \cdot (fF) = f(\nabla \cdot F) + F\cdot \nabla f $$
