## NMM2270.2.5
#### Uses: 
- [[Substitution]]
1. $(x-y)dx +xdy = 0$
Let $y=ux$, $dy = xdu+udx$
$$ (x-\cancel{ux)dx} + (x^2du+\cancel{uxdx})=0 $$
$$ xdx + x^2du = 0 $$
$$ -\frac{x}{x^2}dx = du $$
$$ \int -\frac1xdx=\int du $$
$$ -\ln x + C = u $$
$$ -\ln x+C = \frac yx $$
$$ y = -x\ln x + Cx $$
3. $xdx + (y-2x)dy = 0$
Let $y = ux$, $dy = xdu+udx$
$$ xdx + (ux-2x)(xdu+udx)=0 $$
$$ xdx + ux^2du+u^2xdx-2x^2du-2uxdx=0 $$
$$ ux^2du-2x^2du = -xdx-u^2xdx+2uxdx $$
$$ x^2(udu-2du) = (-x-u^2x+2ux)dx $$
$$ x^2(udu-2du) = (-1-u^2+2u)xdx $$
$$ \frac{udu-2du}{-(u^2-2u+1)} = \frac1xdx $$
$$ \frac{(u-2)}{(u-1)^2}du = -\frac1xdx $$
$$ \frac{(u-1)}{(u-1)^2}du -\frac1{(u-1)^2}du = -\frac1xdx $$
$$ \int\frac1{(u-1)}du - \int\frac{1}{(u-1)^2}du = -\int\frac1xdx $$
$$ \ln|u-1| + \frac1{u-1} = -\ln|x|dx + C $$
$$ \ln|\frac yx-1|+\frac1{\frac yx-1}=-\ln|x|+C $$
5. $(y^2+yx)dx -x^2dy=0$
Let $y=ux$, $dy = udx+xdu$
$$ (u^2x^2 + ux^2)dx - x^2(udx+xdu)=0 $$
$$ u^2x^2dx + \cancel{ux^2dx} - \cancel{ux^2dx} - x^3du=0 $$
$$ x^3du = u^2x^2dx $$
$$ \int\frac1{u^2} = \int\frac1xdx $$
$$ -\frac1u = \ln|x| + C $$
$$ -\frac{x}{y} = \ln|x|+C $$
7. $\frac{dy}{dx} = \frac{y-x}{y+x}$
$$ (y+x)dy = (y-x)dx $$
Let $y = ux$, $dy = udx + xdu$
$$ (ux + x)(udx+xdu) = (ux-x)dx $$
$$ u^2xdx + ux^2du+\cancel{uxdx}+x^2du = \cancel{uxdx} - xdx $$
$$ ux^2du+x^2du = -xdx-u^2xdx $$
$$ x^2(u+1)du = -x(1+u^2)dx $$
$$ \frac{1+u}{1+u^2}du = -\frac1xdx $$
$$ \int\frac{u}{u^2+1}du+\int\frac{1}{1+u^2}du = -\int\frac1xdx $$
$$ \tan^{-1}(u) + \frac12\ln|u^2+1| = -\ln|x| + C $$
$$ \tan^{-1}(\frac yx) + \frac12\ln|\frac{y^2}{x^2}+1| = -\ln|x|+C $$
9. $-ydx + (x+\sqrt{xy})dy = 0$
let $y=ux$, $dy = udx+xdu$
$$ -uxdx+(x+\sqrt{ux^2})(udx+xdu)=0 $$
$$ \cancel{-uxdx}+\cancel{uxdx}+x^2du+u\sqrt{ux^2}dx + x\sqrt{ux^2}du =0 $$
$$ x^2du + x^2\sqrt{u}du = -ux\sqrt{u}dx $$
$$ x^2(1+\sqrt u)du = -u^{\frac32}xdx $$
$$ \frac{-1-u^{\frac12}}{u^{\frac32}} = \frac1xdx $$
$$ -\int\frac1{u^{\frac32}}-\int\frac{1}{u} = \int\frac1xdx $$
$$ 2\frac1{u^\frac12}-\ln|u| = \ln|x| + C $$
$$ \frac2{\sqrt{\frac yx}} - \ln|\frac yx| -\ln|x| = C  $$
$$ -\frac{2\sqrt x}{\sqrt y}+\ln|y| = C $$
$$ -2\sqrt x+\sqrt y\ln|y|= \sqrt y\cdot C $$
$$ -2x+y(\ln|y|)^2 = yC $$
```ad-note
This should be level of simplification
```
11. $xy^2\frac{dy}{dx}=y^3-x^3$ at $y(1) = 2$
$$ xy^2dy = (y^3-x^3)dx $$
Let $y=ux$, $dy = udx+xdu$
$$ x^3u^2(udx+xdu) = (u^3x^3 - x^3)dx $$
$$ \cancel{u^3x^3dx} + u^2x^4du = \cancel{u^3x^3dx} - x^3dx $$
$$ \int u^2du = -\int\frac1xdx $$
$$ \frac13u^3 = -\ln|x| + C $$
$$ u^3+3\ln|x| = C $$
$$ \frac{y^3}{x^3} + \ln|x^3| = C $$
$x = 1$, $y = 2$
$$ \frac{(2)^3}{(1)^3} + \ln|(1)^3| = C $$
$$ 8 + 0 = C $$
$C = 8$
$$ \therefore\frac{y^3}{x^3}+\ln|x^3| = 8 $$
15. $x\frac{dy}{dx} + y = \frac{1}{y^2}$
$$ x\frac{dy}{dx} + y = y^{-2} $$
Let $u = y^{1-(-2)} = y^3$, $y = u^\frac13$, $\frac{dy}{dx} = \frac13u^{-\frac23}\frac{du}{dx}$
$$ x(\frac13u^{-\frac23}\frac{du}{dx}) + u^\frac13 = (u^\frac13)^{-2} $$
$$ \frac13xu^{-\frac23}\frac{du}{dx}+u^\frac13 = u^{-\frac23} $$
Divide by $\frac13xu^{-\frac23}$
$$ \frac{du}{dx} + \frac {3u}x = \frac3x $$
$p(x) = \frac3x$, $q(x) = \frac3x$
$\mu(x) = \int p(x) = 3\ln|x|$
$$ u(x) = e^{-3\ln|x|}\cdot\int e^{3\ln|x|}\cdot\frac3xdx + C\cdot e^{-3\ln|x|} $$
$$ x^{-3}\cdot\int 3\frac{x^3}xdx + C\cdot x^{-3} $$
$$ x^{-3}\cdot x^3 + C\cdot x^{-3} $$
$$ u = 1 + C\cdot x^{-3} $$
$$ y^3 = 1 + C\cdot x^{-3} $$
$$ y = (1+C\cdot x^{-3})^{\frac13} $$
17. $\frac{dy}{dx} = y(xy^3-1)$
$$ \frac{dy}{dx} = xy^4-y $$
$$ \frac{dy}{dx} + y = xy^4 $$
Let $u = y^{1-4} = y^{-3}$, $y = u^{-\frac13}$, $dy = \frac13u^{-\frac43}\frac{du}{dx}$
$$ -\frac13u^{-\frac43}\frac{du}{dx} + u^{-\frac13} = xu^{-\frac43} $$
Divide by $-\frac13u^{-\frac43}$ 
$$ \frac{du}{dx} - 3u = -3x $$
$p(x) = -3$, $q(x) = -3x$
$\mu(x) = -3x$
$$ u = e^{3x}\cdot\int e^{-3x}\cdot3xdx + C\cdot e^{3x} $$
------------- [[Integration by Parts]] -------------
$dv = e^{3x}dx$, $u = 3x$, $du = 3dx$, $v = \frac13e^{3x}$ 
$$ \int e^{3x}\cdot 3xdx = 3x\cdot\frac13e^{3x} - \int\frac13e^{3x}3dx $$
$$ \int e^{3x}\cdot3xdx = xe^{-3x} + \frac13e^{-3x} $$
---------------- IBP --------------------
$$ u = e^{3x}\cdot(xe^{-3x}+\frac13e^{-3x})+C\cdot e^{3x} $$
$$ u = x + \frac13 + C\cdot e^{3x} $$
$$ y^{-3} = \cdots $$
19. $t^2\frac{dy}{dt}+y^2=ty$
$$ \frac{dy}{dt} + \frac{y^2}{t^2}=\frac{y}{t} $$
$$ \frac{dy}{dt} - \frac yt = -\frac{y^2}{t^2} $$
$u = y^{1-(2)} = y^{-1}$, $y = u^{-1}$, $dy = -u^{-2}\frac{du}{dt}$
$$ (-u^{-2})\frac{du}{dt} - \frac1{ut} = -\frac1{u^2t^2} $$
Times by $-u^{2}$ 
$$ \frac{du}{dt}+\frac{u}{t} = \frac1{t^2} $$

$P(t) = \frac{u}{t}$
$Q(t) = \frac1{t^2}$
$\mu(x) = \ln|t|$
$$ u = e^{-\ln|t|}\cdot\int e^{\ln|t|}\cdot\frac{1}{t^2}dt + C\cdot e^{-\ln|t|} $$
$$ u=-t\cdot\int\frac1tdt-tC $$
$$ u=-t\ln|t|-tC $$