### Section 9.14, Problem 3
verify Stokesâ€™ theorem. Assume that the surface S is oriented upward.

$F = zi + xj + yk$; S that portion of the plane $2x + y + 2z = 6$ is in the first octant

Stoke's Theorem:
$$ \oint_{C^+}\vec F\cdot d\vec r = \oint_{C^+}(\vec F \cdot  \vec T)ds = \iint_S (\nabla \times \vec F)\cdot \hat n\;dS $$
### $\iint_S (\nabla \times \vec F)\cdot \hat n\;dS$
Evaluate:
$$ \nabla\times F = \hat i(\frac{\partial F_z}{\partial y} - \frac{\partial F_y}{\partial z})-\hat y(\frac{\partial F_z}{\partial x} - \frac{\partial F_x}{\partial z})+\hat k(\frac{\partial F_y}{\partial x} - \frac{\partial F_x}{\partial y}) $$
$$ \nabla \times F =  (1-0)\hat i - (0-1)\hat j + (1 - 0)\hat k $$
$$ = \hat i + \hat j + \hat k $$
Normal Vector:
$$ g = 2x+y+2z-6 = 0 $$
$$  \hat n = \frac{\nabla g}{|\nabla g|}  $$
$$ \nabla g = \frac{\partial g}{\partial x}\hat i + \frac{\partial g}{\partial y}\hat j + \frac{\partial g}{\partial z}\hat k $$
$$ \nabla g = 2\hat i + 1\hat j + 2\hat k $$
$$ \hat n = \frac{2\hat i + 1\hat j + 2\hat k}{3} = \frac23\hat i + \frac13\hat j + \frac23\hat k $$
$$ \iint_R (\nabla\times F)\cdot \hat nds = \iint_R \frac23 + \frac13 + \frac23ds = \iint_R \frac53ds $$
$$ \iint_R ds = area\; of\; triangle $$
Area:
$$ AB = -3\hat i + 6\hat j + 0\hat k $$
$$ AC = -3\hat i + 0\hat j + 3\hat k $$
area = $\frac{AB \times AC}{2}$
$$ AB\times AC = 
\begin{pmatrix}
\hat i && \hat j && \hat k \\
-3 && 6 && 0 \\
-3 && 0 && 3
\end{pmatrix}
$$
$$ = (18-0)\hat i - (-9-0)\hat j + (0+18)\hat k $$
$$ = 18\hat i + 9\hat j + 18\hat k $$
$$ area = \sqrt{18^2 + 9^2 + 18^2}/2 $$
$$ = \frac{27}2 $$

##### Putting it Together
$$ \iint_R (\nabla\times F)\cdot \hat nds = \frac53\cdot \frac{27}{2} = \frac{45}{2} $$
### $\oint_C F\cdot dr$
$$ dr = dx\hat i + dy\hat j + dz\hat k $$
$$ F\cdot dr = zdx + xdy + ydz $$
$$ \oint_C F\cdot dr = \oint_{C_1} F\cdot dr + \oint_{C_2} F\cdot dr + \oint_{C_3} F\cdot dr $$
Line joining A and C
$$ \frac x3 = \frac y0 = \frac z3 $$
let t = $\frac x3$

$x = 3t, \quad dx = 3dt$
$y = 0\quad dy = 0$
$z = 3t\quad dz = 3dt$

$$ F\cdot dr = 3t\cdot dt + 3t\cdot 0 + 0\cdot 3dt = 9tdt $$
$$ \oint_{C_1} F\cdot dr = 9\int_0^1tdt = \frac92t^2|_0^1 = \frac92 $$
c2:
$$ \frac x3 = \frac y6 = \frac z0 $$
let t = $\frac x3$

$x = 3t\quad dx = 3dt$
$y = 6t\quad dy = 6dt$
$z = 0\quad dz = 0$

$$ F\cdot dr = 18tdt $$
$$ \oint_{C_2} F\cdot dr = 18\int_0^1tdt = 9t^2|_0^1 = 9  $$

c3:
$$ \frac x0 = \frac y6 = \frac z3 $$
let t = $\frac x0$
$x = 0\quad dx = 0$
$y = 6t\quad dy = 6dt$
$z = 3t\quad dz = 3dt$

$$ F\cdot dr = 18tdt $$
$$ \oint_{C_3} F\cdot dr = 18\int_0^1tdt = 9t^2|_0^1 = 9 $$
##### Put it all Together
$$ \oint_C F\cdot dr = \frac92 + 9+9 = \frac{45}2 $$
$\therefore$ theorem is verified



