1. $\mathcal L^{-1}[\frac{1}{s^3}]$
$$ = \frac{t^2}{2} $$
3. $\mathcal L^{-1}[\frac1{s^2}-\frac{48}{s^5}]$
$$ \mathcal L^{-1}[\frac1{s^2}] - \mathcal L^{-1}[\frac{48}{s^5}] = t - 2t^4 $$
5. $\mathcal L^{-1}[\frac{(s+1)^3}{s^4}]$
$(s+1)(s+1)(s+1) = (s+1)(s^2+2s+1) = s^3+2s^2+s+s^2+2s+1 =s^3+3s^2+3s+1$
$$ \mathcal L^{-1}[\frac{s^3}{s^4}] + \mathcal L^{-1}[\frac{3s^2}{s^4}] + \mathcal L^{-1}[\frac{3s}{s^4}]+\mathcal L^{-1}[\frac1{s^4}] $$
$$ = 1 + 3t + \frac32t^2 + \frac16t^3 $$
13. $\mathcal L^{-1}[\frac{4s}{4s^2+1}]$
$$ \mathcal L^{-1}[\frac{4s}{4(s^2+\frac14)}] = \mathcal L^{-1}[\frac{s}{s^2+\frac14}] $$
$$ = \cos(\frac12t) $$
19. $\mathcal L^{-1}[\frac{s}{s^2 + 2s-3}]$
$= \frac{s}{(s+3)(s-1)} = \frac{A}{(s+3)} + \frac{B}{(s-1)}$
$s = As-A + Bs + 3B$
$0 = 3B-A \qquad A = 3B \qquad s = As+Bs = 3Bs+Bs = 4Bs$
$\frac14 = B$
$A = \frac34$
$$ \frac34\mathcal L^{-1}[\frac1{s+3}] + \frac14\mathcal L^{-1}[\frac1{s-1}] $$
$$ \frac34e^{-3t} + \frac14e^{t} $$
Solve using laplace
33. $\frac{dy}{dt} - y = 1$  $y(0) = 0$

$$ \mathcal L[y'] - \mathcal L[y] = \frac1s $$
$$ s\mathcal L[y] - \mathcal L[y] = (s-1)\mathcal L[y] = \frac1s $$
$$ \mathcal L[y] = \frac1{s(s-1)} $$
$= \frac{A}{s} + \frac{B}{s-1} = As - A + Bs = 1$
$A = -1$
$B = 1$
$$ y = \mathcal L^{-1}[-\frac1s] + \mathcal L^{-1}[\frac1{s-1}] $$
$$ y = -1 + e^t $$
