1. $\mathcal L[te^{10t}]$
$$ = \frac1{(s-10)^2} $$
5. $\mathcal L[t(e^t + e^{2t})^2]$
$$ \mathcal L[te^{2t}+2te^{3t} + te^{4t}] =  $$
11. $\mathcal L^{-1}[\frac1{(s+2)^3}]$
$$ = \frac12t^2e^{2t} $$
19. $\mathcal L^{-1}[\frac{2s-1}{s^2(s+1)^3}]$

Solve using laplace transform
21. $y' + 4y = e^{-4t}, \qquad y(0) = 2$
$$ \mathcal L[y'] + 4\mathcal L[y] = \mathcal L[e^{-4t}] $$
$$ s\mathcal L[y] - 2 + 4\mathcal L[y] = \frac{1}{s+4} $$
$$ \mathcal L[y](s+4) = \frac1{s+4}+2 $$
$$ \mathcal L[y] = \frac1{(s+4)^2} + \frac2{(s+4)} $$
$$ y = te^{-4t} + 2e^{-4t} $$

