### 1.
Evaluate the [[Line Integral]] of the function with respect to x, y, and s on the indicated curve
$$ G(x,y) = 2xy \quad x=5\cos t\quad y = 5\sin t\quad 0\leq t\leq \pi/4 $$
With respect to x:
$$ \int_C G(x,y)dx = \int_0^{\frac{\pi}{4}}2xydx $$
$$ = \int_0^{\pi/4}2(5\cos t)(5\sin t)(-5\sin t dt) $$
$$ = -250\int_0^{\pi/4}\cos t\sin^2 t dt $$
U-Sub:
$u = \sin t\qquad du = \cos t dt$
$$ = -250\int_0^{\pi/4}u^2du $$
$$ = -250(\frac{u^3}{3})|_0^{\pi/4} $$
$$ = -\frac{250}3(\sin^3(t))|^{\pi/4}_0 $$
$$ = -\frac{250}{3}((\frac{1}{\sqrt{2}})^3 - 0) $$
$$ = -\frac{250}{3}(\frac{\sqrt{2}}{2})^3 $$
$$ = -\frac{500\sqrt{2}}{24} $$
$$ -\frac{125\sqrt{2}}{6} $$
With respect to y:
$$ \int_C G(x,y)dy = \int_0^{\pi/4}2(5\cos t)(5\sin t)(5\cos t dt) $$
$$ = 250\int_0^{\pi/4}\sin t\cos^2 t dt $$
U Sub:
$$ = -\frac{250}{3}(\cos^3 t)|_0^{\pi/4} $$
$$ = -\frac{250}{3}(\frac{2\sqrt{2}}{8} - 1) $$
$$ = -\frac{125}{6}(4-\sqrt 2) $$
With respect to s:
$ds = \sqrt{(\frac{dx}{dt})^2 + (\frac{dy}{dt})^2}dt$
$ds = \sqrt{25\sin^2t + 25\cos^2t}$
$ds = \sqrt{25(\sin^2t + \cos^2t)}$
$ds = 5dt$
$$ \int_C G(x,y)ds = \int_0^{\pi/4}2(5\cos t)(5\sin t)(5dt) $$
$$ = 250 \int_0^{\pi/4}\cos t\sin tdt $$
$$ = \frac{250}2(\sin^2 t)|^{\pi/4}_0 $$
$$ = 125(\frac{\sqrt{2}}{2})^2 $$
$$ = \frac{125}{2} $$
### 3.
Evaluate the [[Line Integral]] of the function with respect to x, y, and s on the indicated curve
$$ G(x,y) = 3x^2+6y^2\qquad y = 2x+1\qquad -1\leq x\leq 0 $$
$$ \int_C G(x,y)dx = \int_{-1}^0 3x^2 + 6(2x+1)^2dx $$
$$ = \int_{-1}^03x^2 + 6(4x^2 + 4x + 1)dx $$
$$ = \int_{-1}^0 3x^2 + 24x^2 + 24x + 6dx $$
$$ = (x^3)|_{-1}^0 + 8(x^3)|_{-1}^0 + 12(x^2)|_{-1}^0 + 6(x)|_{-1}^0 $$
$$ = (-1 - 0) + 8(-1 - 0) + 12(1 - 0) + 6(-1-0) $$
$$ = -1 - 8 + 12 - 6 $$
$$ = -3 $$
$$ \int_C G(x,y)dy = \int_{-1}^03x^2 + 6(2x+1)^2dy $$
$dy = \frac{dy}{dx}(2x+1)$
$dy = 2dx$
$$ = \int_{-1}^0 (3x^2 + 6(4x^2 + 4x + 1))2dx $$
$$ = 2((x^3)|_{-1}^0 + 8(x^3)|_{-1}^0 + 12(x^2)_{-1}^0 + 6(x)|_{-1}^0) $$
$$ = 2((-1 - 0) + 8(-1 - 0) + 12(1-0) + 6(-1 - 0)) $$
$$ = 2(-1-8+12-6) $$
$$ = -6 $$
Both -3 and -6 are supposed to be +. Its supposed to be x=0 - x=-1. I did it backwards here
$$ \int_C G(x,y)ds = \int_{-1}^0 (3x^2 + 6(4x^2 + 4x + 1))ds $$
$ds = \sqrt{1+(\frac{dy}{dx})^2}dx$
$ds = \sqrt 5dx$
$$ = \int(3\sqrt 5x^2 + 24\sqrt5x^2 + 24\sqrt5x + 6\sqrt5)dx $$
$$ = \int_{-1}^0 27\sqrt 5x^2 + \int_{-1}^024\sqrt 5x + \int_{-1}^06\sqrt 5 $$
$$ = 9\sqrt 5(0 + 1) + 12\sqrt5(0-1) + 6\sqrt 5(0+1) $$
$$ = 9\sqrt 5 - 12\sqrt 5 + 6\sqrt 5 $$
$$ = 3\sqrt 5 $$
### 32.
Find the work done by the force $F(x,y) = 2xy\hat i + 4y^2\hat j$ acting along the piecewise smooth curve consisting of line segments from (-2,2) to (0,0) and from (0,0) to (2,3)
$$ \int_C F\cdot dr = \int_{C_1} F\cdot dr + \int_{C_2}F\cdot dr $$
Line Segment 1: $y = -x = g \qquad x = x = f$
Line Segment 2: $y = \frac{3}{2}x = g\qquad x=f$
Calculate $dr$:
$dr_1 = f'\hat i + g'\hat j = 1\hat i - 1\hat j$
$dr_2 = 1\hat i + \frac{3}{2}\hat j$
$$ = \int_{-2}^0((-2x^2\hat i + 4x^2\hat j)\cdot (\hat i - \hat j)) + \int_0^2((3x^2\hat i + 9x^2\hat j)\cdot (\hat i + \frac32\hat j)) $$
$$ = \int_{-2}^0(-2x^2 - 4x^2) + \int_0^2(3x^2 + \frac{27}{2}x^2) $$
$$ = \int_{-2}^0(-6x^2) + \int_0^2(\frac{33}{2}x^2) $$
$$ = (-2x^3)|_{-2}^0 + (\frac{11}{2}x^3)|_0^2 $$
$$ = (0-16) + \frac{11}{2}(8-0) $$
$$ =-16 + 44 $$
$$ = 28 $$
### 33.
Find the work done by the force $F(x,y) = (x+2y)\hat i + (6y-2x)\hat j$ acting counterclockwise once around the triangle with vertices (1,1),(3,1), and (3,2)
![[Drawing 2023-04-23 22.39.24.excalidraw]]

##### $C_1$:
dependent on x ($1\to 3$)
$y = 1 = g$
$dr = 1\hat i + 0\hat j$
$F\cdot dr = ((x+2)\hat i + (6-2x)\hat j)\cdot(\hat i + 0\hat j)$
$F\cdot dr = x+2$

##### $C_2$:
dependent on y ($1\to 2$)
$x = 3$
$dr = 0\hat i + 1\hat j$
$F\cdot dr = ((3+2y)\hat i + (6y-6)\hat j)\cdot (0\hat i + \hat j)$
$F\cdot dr = 6y - 6$

##### $C_3$:
dependent on x ($3\to 1$)
$y = \frac{1}{2}x + \frac12$
$dr = \hat i + \frac12\hat j$
$F\cdot dr = ((x + x + 1)\hat i + (3x + 3 - 2x)\hat j)\cdot (\hat i + \frac12\hat j)$
$F\cdot dr = 2x+1 + \frac12x + \frac32$
$F\cdot dr = \frac52x + \frac52$

$$ = \int_1^3(x+2) + \int_1^2(6y-6) + \int_3^1(\frac52x + \frac52) $$
$$ = (\frac12x^2 + 2x)|_1^3 + (3y^2 - 6y)|_1^2 + (\frac54x^2 + \frac52x)|_3^1 $$
$$ = (\frac92 + 6 - \frac12 - 2) + (12 - 12 - 3+6) + (\frac54 + \frac52 - \frac{45}4 - \frac{15}2) $$
$$ = 8 + 3 + (-10 - 5) $$
$$ = -4 $$
Could have also solved by making x and y a function of $t$





