1. $\mathcal L[te^{-10t}]$
$$ F(s) = \frac{1}{s+10} $$
$$ \mathcal L[te^{-10t}] = (-1)(-1)\frac1{(s+10)^2} = \frac{1}{(s+10)^2} $$
11. $y'' + 9y = \cos(3t), \qquad y(0) = 2, y'(0) = 5$
$$ \mathcal L[y''] + 9\mathcal L[y] = \frac{s}{s^2 + 9} $$
$$ s^2\mathcal L[y] - 2s -5 + 9\mathcal L[y] = \frac{s}{s^2+9} $$
$$ \mathcal L[y](s^2+9) = \frac{s}{s^2+9} -2s -5 $$
$$ \mathcal L[y] = \frac{s}{(s^2+9)^2} - 2\frac{s}{s^2+9} - \frac{5}{s^2+9} $$
$$ \mathcal L^{-1}[\frac{s}{(s^2+9)^2}] = -t\cos(3t) $$
23. $\mathcal L[1*t^3]$
$$ \mathcal L[1*t^3] = \mathcal L[1]\mathcal L[t^3] $$
$$ = \frac1s\cdot\frac6{s^4} = \frac6{s^5} $$