---
date-created: 2022-09-16
concepts: "seperable-differential-equations", "trig-identities"
---
Concepts: 
- [[Seperable Differential Equations]]
- [[Trig Identities]]
## NMM 2270 2.2 Practice Problems
1. $\frac{dy}{dx} = \sin5x$
$$\int dy = \int \sin5x\;dx $$
$$ y = -\frac{1}{5}\cos5x + C $$
3. $dx + e^{3x}dy=0$
$$ \int-e^{-3x}dx = \int dy $$
$$ \frac{1}{3}e^{-3x} + C= y $$
5. $x\frac{dy}{dx} = 4y$
$$ \int\frac{dy}{y} = \int\frac{4dx}{x} $$
$$ \ln|y| = 4\ln|x| + C $$
$$ \ln|y| = \ln|x^4| + C $$
$$ \ln|y| = \ln|x^4| + \ln|e^C| $$
$$ \ln|y| = \ln(e^C|x^4|) $$
$$ |y| = C|x^4| $$
$$ y = Cx^4 $$
7. $\frac{dy}{dx} = e^{3x + 2y}$
$$ \frac{dy}{dx} = e^{3x}e^{2y} $$
$$ \int e^{-2y}dy = \int e^{3x}dx $$
$$ -3e^{-2y} = 2e^{3x} $$
9. $y\ln x\frac{dy}{dx} = (\frac{y+1}{x})^2$
$$ \frac{dy}{dx} = (\frac{y+1}{x})^2\frac{1}{y\ln x} $$
$$ \frac{dy}{dx} = \frac{y^2 + 2y + 1}{x^2}\frac{1}{y}\frac{1}{\ln x} $$
$$ \frac{dy}{dx} = \frac{y^2 + 2y + 1}{y}\frac{1}{x^2\ln x} $$
$$ \frac{dy}{dx} = (y + 2 + \frac{1}{y})\frac{1}{x^2\ln x} $$
$$ \int(y + 2 + \frac1y)dy = \int\frac{dx}{x^2\ln x} $$
$$ \frac{1}{2}y^2 + 2y + \ln y =  $$
```ad-question
How to Integrate Right Side? [[Integration by Parts]]? [[Integrals of Rational Functions]]?  Left half is correct
```
11. $\csc ydx + \sec^2xdy = 0$
$$ \csc ydx = -\sec^2xdy $$
$$ \csc y = -\sec^2x \frac{dy}{dx} $$
$$ \int\frac{dx}{-\sec^2x} = \int\frac{dy}{\csc y} $$
$$ \int-\cos^2x dx = \int \sin y dy $$
$$ -\frac12x - \frac14\sin2x + C = -\cos y $$
$$ \frac12x + \frac14\sin2x+C = \cos y $$
$$ 2x + \sin2x + C = 4\cos y $$
13. $(e^y+1)^2e^{-y}dx + (e^x + 1)^3e^{-x}dy = 0$
$$ (e^y + 1)^2e^{-y} = (e^x+1)^3e^{-x}\frac{dy}{dx} $$
$$ \frac{(e^y+1)^2e^{-y}}{(e^x + 1)^3e^{-x}} = \frac{dy}{dx} $$
$$ \int\frac{e^xdx}{(e^x + 1)^3} = \int\frac{e^ydy}{(e^y+1)^2} $$
$$ -\frac12\frac{1}{(e^x + 1)^{2}} = -\frac{1}{(e^y+1)} $$
15. $\frac{dS}{dr} = kS$
$$ \int\frac{dS}{S} = \int kdr $$
$$ \ln(S) = kr + C $$
$$ S = Ce^{kr} $$
17. $\frac{dP}{dt} = P - P^2$ **
$$ \int \frac{dP}{P-P^2} = \int dt $$
$$ \int\frac{dP}{P(1-P)} = t $$
--------------------------------------------------------
$$ \frac{A}{P} + \frac{B}{1-P} = \frac1{P(1-P)} $$
$$ A-AP +BP = 1 $$
$$ (B-A)P + A = 1 $$
B = A     A = 1
------------------------------------------------------------------------------------
$$ \int\frac{dP}{P} - \int\frac{dP}{1-P} = t $$
$$ \ln P - \ln(1-P) = t + C $$
$$ P - 1 + P = Ce^t $$
19. $\frac{dy}{dx} = \frac{xy+3x-y-3}{xy-2x+4y-8}$
$$ \frac{dy}{dx} = \frac{x(y+3)-1(y+3)}{x(y-2)+4(y-2)} $$
$$ \frac{dy}{dx} = \frac{(y+3)(x-1)}{(y-2)(x+4)} $$
$$ \int\frac{(y-2)dy}{(y+3)} = \int\frac{(x-1)dx}{(x+4)} $$
add +3-3 and +4-4
$$ \int\frac{(y+3)-2-3}{(y+3)}dy = \int\frac{(x+4)-4-1}{(x+4)}dx $$
$$ \int dy -5 \int\frac1{y+3}dy = \int dx-5\int\frac1{x+4} $$
$$ y - 5\ln(y+3) = x -5\ln(x+4) $$
21. $\frac{dy}{dx} = x\sqrt{1-y^2}$
$$ \int \frac{dy}{\sqrt{1-y^2}} = \int xdx $$
$$ \sin^{-1}y = \frac12x^2 + C $$
23. $\frac{dx}{dt} = 4(x^2 + 1)$, $x(\frac{\pi}4) = 1$

$$ \int\frac{dx}{x^2 + 1} = \int4dt $$
$$ -\cot^{-1}x = 4t + C $$
$$ x = \cot(-4t + C) $$
sub in
$$ 1 = \cot(-1 +C) $$
$$ \cot^{-1}(1) = -1 + C $$