### Theorem
Given $a_0(x), a_1(x),\cdots, a_n(x)$, where $a_n(x) \neq 0$ and F(x) are continuous. And given a, $b_0$, $b_1$, $\cdots$, $b_{n-1}$ are real numbers
$$  a_n(x)y^{(n)}(x) + a_{n-1}(x)y^{(n-1)}(x) + \cdots + a_1(x)y^{(1)}(x) + a_0(x)y^{(0)}(x) = F(x)  $$
$$ y(a) = b_0,\; y^{(1)}(a) = b_1,\; y^{(2)}(a) = b_2, \cdots,y^{(n-1)}(a) = b_{n-1} $$

If n = 2
$$ y(x) = C_1y_1(x) + C_2y_2(x) $$
$y_1(x)$ and $y_2(x)$ is [[linearly independent]]

Iinital Conditions (I.C)
$$ y(a) = b_0 = C_1y_1(a) + C_2y_2(a) $$
$$ y'(a) = b_1 = C_1y'_1 + C_2y'_2(a) $$
