#### Question 2
$$ y^{(3)}-2y''-y'+2y = 24e^{2t} $$
Homogenous Part
$$ r^3-2r^2-r+2 = 0 $$
$$ r^2(r-2)-(r-2) = (r-2)(r^2-1) $$
$r_1 = 2$
$r_2 = -1$
$r_3 = 1$
$$ y_c = C_1e^{2x} + C_2e^{-x}+C_3e^x $$
$$ y_p = Bte^{2t} $$
$$ y'_p = Be^{2t} + 2Bte^{2t} $$
$$ y_p'' = 2Be^{2t} + 2Be^{2t} + 4Bte^{2t} $$
$$ y_p'' = 4Be^{2t} + 4Bte^{2t} $$
$$ y_p''' = 4Be^{2t} + 4Be^{2t}+4Be^{2t}+8Bte^{2t} $$
$$ y'''_p = 12Be^{2t} + 8Bte^{2t} $$
sub these ^ into base equation:
$$ e^{2t}(12B+8Bt -4B-4B-4Bt-B-2B+2Bt) = 24e^{2t} $$
$$ B + 6Bt = 24 $$

$$ (12B-8B-B) + (8Bt-8Bt-2Bt+2Bt) = 24 $$
$$ 3B = 24 $$
$$ y =  C_1e^{2x} + C_2e^{-x}+C_3e^x + 8te^{2t} $$
$$ 4 = C_1 + C_2 + C_3 $$
$$ y' = 2C_1e^{2t} - C_2e^{-x}+C_3e^x+8e^{2t}+16te^{2t} $$
$$ 9 = 2C_1-C_2+C_3+8 $$
$$ y'' = 4C_1e^{2t}+C_2e^{-x}+C_3e^x+16e^{2t}+16e^{2t}+32te^{2t} $$
$$ 3 = 4C_1 + C_2+C_3+32 $$


### 3
a. 
$$ y_p = [(A_1x+A_2)(Be^x)] + (C_1\sin x + C_2\cos x) $$
b.
$$ y_p = (A_1x^2+A_2x+A_3)+(B)+(C_1\sin2x + C_2\cos2x) $$
c.
$$ y_p = [(A_1t+A_2)(B_1\sin2t + B_2\cos2t)] + [(C_1t^2 + C_2t+C_2)(De^{-t})]  $$
